add alt version in Conditional_Loop to illustrate an issue

boogie_examples/Conditional_Loop.bpl
@@ -3,11 +3,13 @@
 This example was done in BoogieExamples.bpl but the encoding
 is a little ad hoc (simplified in ways that make it 
 non-obvious that it's in accord with the standard translation).
+
 This file again starts from the WhyRel
 version (copied below) but encodes it more closely to the 
-WhyRel encoding of bi-while.
+WhyRel encoding of bi-while which is 
+all_exists/Conditional_Loop/prog.rl.
 
-all_exists/Conditional_Loop/prog.rl 
+In fact we do two versions, to illustrate a technical point.
 
   meth m (x:int, n: int | x:int, n: int) : (int|int)
     requires { Both(n > 0) }
@@ -35,7 +37,12 @@ all_exists/Conditional_Loop/prog.rl
     |_ result := z _|;
  */
 
-procedure loop (x1: int, n1: int, x2: int, n2: int)
+/* First version: simple non-exclusive alignment conditions; fails
+   to verify unless the RO snapshot include exclusion condition.
+   We add it here --see NOTE-- but that diverges from def of chk
+   function for filter-adequacy. */
+
+procedure loop1 (x1: int, n1: int, x2: int, n2: int)
   returns (z1: int, z2: int)
 
   requires n1 > 0 && n2 > 0;
@@ -87,7 +94,8 @@ procedure loop (x1: int, n1: int, x2: int, n2: int)
     // snapshot variant [> (n - w) mod n >] (added by chk)
     vnt := (n2 - w2) mod n2;
     // snapshot RO condition (added by chk)
-    ro := (y2 > 0 && w2 != 0) && !(y1 > 0 && w1 != 0);
+    ro := (y2 > 0 && w2 != 0) 
+         && !(y1 > 0 && w1 != 0); // NOTE: not really added by chk
 
     // left-only condition
     if (y1 > 0 && w1 != 0)
@@ -96,7 +104,109 @@ procedure loop (x1: int, n1: int, x2: int, n2: int)
        { havoc z1; y1 := y1 - 1; }
        w1 := (w1 + 1) mod n1; 
     } 
+    // right-only condition 
     else if (y2 > 0 && w2 != 0)
+    {  // bi-right projection of body
+       if (w2 == 0)
+       { assert (exists v: int :: z1 == v); // added by chk
+         havoc z2; // HavocR z { z := z }
+         assume z1 == z2;    
+         y2 := y2 - 1; 
+       }
+       w2 := (w2 + 1) mod n2;         
+     }
+     else 
+     { // an alignment of body
+       assert w1 == 0 <==> w2 == 0;
+       if (w1 == 0 && w2 == 0)
+       {
+         havoc z1; // (havoc z | skip)
+         assert (exists v: int :: z1 == v); // added by chk
+         havoc z2; // HavocR z { z := z }
+         assume z1 == z2;
+         y1 := y1 - 1; y2 := y2 - 1; // |_ y := y - 1 _|
+       } 
+       // |_ w := (w + 1) mod n _|
+       w1 := (w1 + 1) mod n1; w2 := (w2 + 1) mod n2;
+     } 
+
+    // variant decreases and lower bounded on RO (added by chk)
+    assert ro ==> (0 <= ((n2 - w2) mod n2));
+    assert ro ==> ((n2 - w2) mod n2) < vnt; // NOTE: fails without NOTE above
+  }
+}
+
+
+
+
+/* Second version: formulate the alignment conditions to be 
+   mutually exclusive, and strictly follow the RO snapshot in 
+   def of chk for filter-adequacy. */
+
+procedure loop2 (x1: int, n1: int, x2: int, n2: int)
+  returns (z1: int, z2: int)
+
+  requires n1 > 0 && n2 > 0;
+  requires x1 >= 0 && x2 >= 0;
+  requires x1 == x2;
+  ensures z1 == z2;
+{
+
+  var y1: int; var y2: int;
+  var w1: int; var w2: int;
+
+  // locals for snapshots
+  var ro: bool;
+  var vnt: int;
+
+  y1 := x1; y2 := x2; // |_ y := x _|
+  z1 := 0;  z2 := 0;  // |_ z := 0 _|
+  w1 := 0;  w2 := 0;  // |_ w := 0 _|
+
+  // While (y > 0) | (y > 0) . 
+  //    <| w <> 0 <] | !(y1 > 0 && w1 <> 0) && [> w <> 0 |> do
+  while (y1 > 0 || y2 > 0)
+    // y =:= y
+    invariant y1 == y2;
+
+    // Both (0 <= y /\ y <= x)
+    invariant 0 <= y1 && y1 <= x1;
+    invariant 0 <= y2 && y2 <= x2;
+
+    // Both (0 <= w /\ w < n)
+    invariant 0 <= w1 && w1 < n1;
+    invariant 0 <= w2 && w2 < n2;
+
+    // z =:= z
+    invariant z1 == z2;
+
+    // adequacy of the loop
+    invariant (
+      // LO
+      (y1 > 0 && w1 != 0) ||
+      // RO
+      (y2 > 0 && w2 != 0) ||
+      // JO
+      (y1 > 0 && y2 > 0 && w1 == 0 && w2 == 0) ||
+      // done
+      (y1 <= 0 && y2 <= 0)
+    );
+  {
+
+    // snapshot variant [> (n - w) mod n >] (added by chk)
+    vnt := (n2 - w2) mod n2;
+    // snapshot RO condition (added by chk)
+    ro := (y2 > 0 && w2 != 0 && !(y1 > 0 && w1 != 0));
+
+    // left-only condition
+    if (y1 > 0 && w1 != 0)
+    {  // left projection of body
+       if (w1 == 0)
+       { havoc z1; y1 := y1 - 1; }
+       w1 := (w1 + 1) mod n1; 
+    } 
+    // right-only condition 
+    else if (y2 > 0 && w2 != 0 && !(y1 > 0 && w1 != 0))
     {  // bi-right projection of body
        if (w2 == 0)
        { assert (exists v: int :: z1 == v); // added by chk
